@prefix apn: <https://w3id.org/apn/> .
@prefix dce: <http://purl.org/dc/elements/1.1/> .
@prefix dct: <http://purl.org/dc/terms> .
@prefix dpv: <http://www.w3.org/ns/dpv#> .
@prefix owl: <http://www.w3.org/2002/07/owl#> .
@prefix rdfs: <http://www.w3.org/2000/01/rdf-schema#> .
@prefix skos: <http://www.w3.org/2004/02/skos/core#> .
@prefix vann: <http://purl.org/vocab/vann/> .
@prefix xsd: <http://www.w3.org/2001/XMLSchema#> .

dpv:Age rdfs:subClassOf apn:Personalisation .

dpv:Authenticating rdfs:subClassOf apn:Personalisation .

dpv:BrowsingBehavior rdfs:subClassOf apn:Personalisation .

dpv:DeviceBased rdfs:subClassOf apn:Personalisation .

dpv:EthnicOrigin rdfs:subClassOf apn:Personalisation .

dpv:FamilyStructure rdfs:subClassOf apn:Personalisation .

dpv:Interest rdfs:subClassOf apn:Personalisation .

dpv:Location rdfs:subClassOf apn:Personalisation .

dpv:MedicalHealth rdfs:subClassOf apn:Personalisation .

dpv:PoliticalAffiliation rdfs:subClassOf apn:Personalisation .

dpv:Professional rdfs:subClassOf apn:Personalisation .

dpv:PurchasesAndSpendingHabit rdfs:subClassOf apn:Personalisation .

dpv:SocialNetwork rdfs:subClassOf apn:Personalisation .

apn: a owl:Ontology ;
    dce:creator "Beatriz Esteves", "Kieran Fraser", "Shridhar Kulkarni" ;
    dct:created "2022-02-16"^^xsd:date ;
    dct:license <http://purl.org/NET/rdflicense/cc-by4.0> ;
    dce:title "Ontology for the Annotation of Push-Notifications" ;
    vann:preferredNamespacePrefix "apn:"^^xsd:string ;
    vann:preferredNamespaceUri "https://w3id.org/apn/"^^xsd:string ;
    dct:modified "2022-06-24"^^xsd:date ;
    owl:versionInfo "0.2"^^xsd:string .

apn:AccountManagement a owl:Class ;
    rdfs:label "Account Management" ;
    skos:definition "Notifications that encourage subscribers to create and/or log into an account to take advantage of a certain feature."@en ;
    rdfs:subClassOf apn:CallToAction .

apn:ArtAndDesign a owl:Class ;
    rdfs:label "Art And Design" ;
    rdfs:subClassOf apn:ApplicationType .

apn:Awareness a owl:Class ;
    rdfs:label "Awareness" ;
    skos:definition "The notification makes subscribers aware of information that does not need further investigation by the subscriber, e.g., a new feature, upcoming holiday, weather, stock price, score in a match, etc. "@en ;
    rdfs:subClassOf apn:CallToAction .

apn:Beauty a owl:Class ;
    rdfs:label "Beauty" ;
    rdfs:subClassOf apn:ApplicationType .

apn:BooksAndReference a owl:Class ;
    rdfs:label "Books And Reference" ;
    rdfs:subClassOf apn:ApplicationType .

apn:Business a owl:Class ;
    rdfs:label "Business" ;
    rdfs:subClassOf apn:ApplicationType .

apn:CT_Awareness a owl:Class ;
    rdfs:label "Campaign Type: Awareness" ;
    skos:definition "A campaign to promote general awareness of a topic."@en ;
    rdfs:subClassOf apn:CampaignType .

apn:CT_BreakingContent a owl:Class ;
    rdfs:label "Campaign Type: Breaking Content" ;
    skos:definition "A campaign to promote new content that has just been created."@en ;
    rdfs:subClassOf apn:CampaignType .

apn:CT_HelpFeedbackTips a owl:Class ;
    rdfs:label "Campaign Type: Help Feedback Tips" ;
    skos:definition "A campaign to get help or tips and to provide feedback."@en ;
    rdfs:subClassOf apn:CampaignType .

apn:CT_Loyalty a owl:Class ;
    rdfs:label "Campaign Type: Loyalty" ;
    skos:definition "A campaign directed at loyal / returning / engaged users or customers."@en ;
    rdfs:subClassOf apn:CampaignType .

apn:CT_Newsletter a owl:Class ;
    rdfs:label "Campaign Type: Newsletter" ;
    skos:definition "Informative campaign containing 'things of interest' to the user."@en ;
    rdfs:subClassOf apn:CampaignType .

apn:CT_Onboarding a owl:Class ;
    rdfs:label "Campaign Type: Onboarding" ;
    skos:definition "A campaign to induct users with a product/service, to acquaint them with features available or account management."@en ;
    rdfs:subClassOf apn:CampaignType .

apn:CT_Product a owl:Class ;
    rdfs:label "Campaign Type: Product" ;
    skos:definition "A campaign to promote a particular product/feature."@en ;
    rdfs:subClassOf apn:CampaignType .

apn:CT_PromotionalFlash a owl:Class ;
    rdfs:label "Campaign Type: Promotional Flash" ;
    skos:definition "A campaign to promote flash sale offers, i.e., they have some time limit associated."@en ;
    rdfs:subClassOf apn:CT_Promotional .

apn:CT_PromotionalGeneral a owl:Class ;
    rdfs:label "Campaign Type: Promotional General" ;
    skos:definition "A campaign to promote general offers for the users."@en ;
    rdfs:subClassOf apn:CT_Promotional .

apn:CT_PromotionalRare a owl:Class ;
    rdfs:label "Campaign Type: Promotional Rare" ;
    skos:definition "A campaign to promote a service/product associated with particular seasons and/or holidays/events."@en ;
    rdfs:subClassOf apn:CT_Promotional .

apn:CT_Reengagement a owl:Class ;
    rdfs:label "Campaign Type: Reengagement" ;
    skos:definition "A campaign enticing users / customers to re-engage with the service."@en ;
    rdfs:subClassOf apn:CampaignType .

apn:CT_Social a owl:Class ;
    rdfs:label "Campaign Type: Social" ;
    skos:definition "A campaign based on or associated with social tools, social media or influencers."@en ;
    rdfs:subClassOf apn:CampaignType .

apn:Claim a owl:Class ;
    rdfs:label "Claim" ;
    skos:definition "Notifications that encourage the subscribers to click and claim some prize or reward from the application."@en ;
    rdfs:subClassOf apn:CallToAction .

apn:Comics a owl:Class ;
    rdfs:label "Comics" ;
    rdfs:subClassOf apn:ApplicationType .

apn:Communication a owl:Class ;
    rdfs:label "Communication" ;
    rdfs:subClassOf apn:ApplicationType .

apn:Country a owl:Class ;
    rdfs:label "Country" ;
    skos:definition "Targeting users based on their country of residence."@en ;
    rdfs:subClassOf apn:Geographic .

apn:Discover a owl:Class ;
    rdfs:label "Discover" ;
    skos:definition "Notifications that tease the content of the information itself to generate curiosity on the users and lead them to engage with the app."@en ;
    rdfs:subClassOf apn:CallToAction .

apn:Download a owl:Class ;
    rdfs:label "Download" ;
    skos:definition "Notifications to get the subscriber to download some asset."@en ;
    rdfs:subClassOf apn:CallToAction .

apn:Education a owl:Class ;
    rdfs:label "Education" ;
    rdfs:subClassOf apn:ApplicationType .

apn:Engagement a owl:Class ;
    rdfs:label "Engagement" ;
    skos:definition "Targeting users based on their engagement with the app, e.g., they have liked a video, followed another user, started a game."@en ;
    rdfs:subClassOf apn:Behavior .

apn:Entertainment a owl:Class ;
    rdfs:label "Entertainment" ;
    rdfs:subClassOf apn:ApplicationType .

apn:Events a owl:Class ;
    rdfs:label "Events" ;
    rdfs:subClassOf apn:ApplicationType .

apn:FamilyStatus a owl:Class ;
    rdfs:label "Family Status" ;
    skos:definition "Targeting users based on their family status, e.g., new parents, pregnancies."@en ;
    rdfs:subClassOf apn:Demographic .

apn:Feedback a owl:Class ;
    rdfs:label "Feedback" ;
    skos:definition "Notifications to get the subscriber to provide some form of feedback or response, for instance on the app's functionalities."@en ;
    rdfs:subClassOf apn:CallToAction .

apn:Finance a owl:Class ;
    rdfs:label "Finance" ;
    rdfs:subClassOf apn:ApplicationType .

apn:FoodAndDrink a owl:Class ;
    rdfs:label "Food And Drink" ;
    rdfs:subClassOf apn:ApplicationType .

apn:Games a owl:Class ;
    rdfs:label "Games" ;
    rdfs:subClassOf apn:ApplicationType .

apn:Health a owl:Class ;
    rdfs:label "Health" ;
    skos:definition "Targeting users based on their health status."@en ;
    rdfs:subClassOf apn:Demographic .

apn:HealthAndFitness a owl:Class ;
    rdfs:label "Health And Fitness" ;
    rdfs:subClassOf apn:ApplicationType .

apn:HolidayDuration a owl:Class ;
    rdfs:label "Duration of holiday" ;
    skos:definition "The notification is likely only relevant leading up to, during or just after a holiday period (e.g. Christmas, Father's Day, International Earth Day, World Radio Day, International Women's Day etc.)"@en ;
    rdfs:subClassOf apn:Urgency .

apn:Interest a owl:Class ;
    rdfs:label "Interest" ;
    skos:definition "Targeting users based on their interests, personal motivations or lifestyle."@en ;
    rdfs:subClassOf apn:Psychographic .

apn:Job a owl:Class ;
    rdfs:label "Job" ;
    skos:definition "Targeting users who have a particular interest, e.g., football goal updates indicates an interest in sports and a new recipe an interest in cooking."@en ;
    rdfs:subClassOf apn:Demographic .

apn:LibrariesAndDemo a owl:Class ;
    rdfs:label "Libraries And Demo" ;
    rdfs:subClassOf apn:ApplicationType .

apn:Lifestyle a owl:Class ;
    rdfs:label "Lifestyle" ;
    skos:definition "Targeting users based on their particular lifestyle, e.g., vegan products, a person who runs or works out."@en ;
    rdfs:subClassOf apn:ApplicationType,
        apn:Psychographic .

apn:Loyalty a owl:Class ;
    rdfs:label "Loyalty" ;
    skos:definition "Targeting a segment of users who are particularly loyal, e.g., daily recurrent users."@en ;
    rdfs:subClassOf apn:Behavior .

apn:MapsAndNavigation a owl:Class ;
    rdfs:label "Maps And Navigation" ;
    rdfs:subClassOf apn:ApplicationType .

apn:Medical a owl:Class ;
    rdfs:label "Medical" ;
    rdfs:subClassOf apn:ApplicationType .

apn:Motivation a owl:Class ;
    rdfs:label "Motivation" ;
    skos:definition "Targeting users based on their aspirations or motivations, e.g., find a new job, get fitter, learn a new skill."@en ;
    rdfs:subClassOf apn:Psychographic .

apn:MusicAndAudio a owl:Class ;
    rdfs:label "Music And Audio" ;
    rdfs:subClassOf apn:ApplicationType .

apn:NewsAndMagazines a owl:Class ;
    rdfs:label "News And Magazines" ;
    rdfs:subClassOf apn:ApplicationType .

apn:Days a owl:Class ;
    rdfs:label "Days" ;
    skos:definition "The notification is likely only relevant within a number of days within the next week."@en ;
    rdfs:subClassOf apn:Urgency .

apn:Hours a owl:Class ;
    rdfs:label "Hours" ;
    skos:definition "The notification is likely only relevant within a number of hours in the current day."@en ;
    rdfs:subClassOf apn:Urgency .

apn:Minutes a owl:Class ;
    rdfs:label "Minutes" ;
    skos:definition "The notification is likely only relevant within a number of minutes in the current hour."@en ;
    rdfs:subClassOf apn:Urgency .

apn:Weeks a owl:Class ;
    rdfs:label "Weeks" ;
    skos:definition "The notification is likely only relevant within a number of weeks."@en ;
    rdfs:subClassOf apn:Urgency .

apn:Occasion a owl:Class ;
    rdfs:label "Occasion" ;
    skos:definition "Targeting users who have engaged with or expressed interest in rare events, e.g., previously purchased during a holiday."@en ;
    rdfs:subClassOf apn:Behavior .

apn:PersonalMotivations a owl:Class ;
    rdfs:label "Personal Motivations" ;
    skos:definition "Information about personal motivations."@en ;
    rdfs:subClassOf apn:Personalisation .

apn:Photography a owl:Class ;
    rdfs:label "Photography" ;
    rdfs:subClassOf apn:ApplicationType .

apn:Play a owl:Class ;
    rdfs:label "Play" ;
    skos:definition "Notifications related with gaming apps, where the subscriber is encouraged to re-engage with the game."@en ;
    rdfs:subClassOf apn:CallToAction .

apn:Product a owl:Class ;
    rdfs:label "Product" ;
    skos:definition "Targeting users who have engaged with or expressed interest in a specific product, e.g., you will love the new X product just launched."@en ;
    rdfs:subClassOf apn:Behavior .

apn:Productivity a owl:Class ;
    rdfs:label "Productivity" ;
    rdfs:subClassOf apn:ApplicationType .

apn:Purchase a owl:Class ;
    rdfs:label "Purchase" ;
    skos:definition "Notifications to get the subscriber to purchase a product or service."@en ;
    rdfs:subClassOf apn:CallToAction .

apn:PurchasingReason a owl:Class ;
    rdfs:label "Purchasing Reason" ;
    skos:definition "Targeting users who have previously purchased or require a reason, incentive or nudge to purchase, e.g., you previously bought X, we recommend Y; 30% sale on now."@en ;
    rdfs:subClassOf apn:Behavior .

apn:Region a owl:Class ;
    rdfs:label "Region" ;
    skos:definition "Targeting users based on their geographic region, i.e., a location within a country."@en ;
    rdfs:subClassOf apn:Geographic .

apn:Reminder a owl:Class ;
    rdfs:label "Reminder" ;
    skos:definition "Notifications that serve as a reminder or alert to the users or provide advice / tips."@en ;
    rdfs:subClassOf apn:CallToAction .

apn:Residence a owl:Class ;
    rdfs:label "Residence" ;
    skos:definition "Targeting users based on their type of residence, e.g., their house contains a garden."@en ;
    rdfs:subClassOf apn:Demographic .

apn:SeasonDuration a owl:Class ;
    rdfs:label "Duration of season" ;
    skos:definition "The notification is likely only relevant during a season e.g. Winter, Summer, Autumn, Spring."@en ;
    rdfs:subClassOf apn:Urgency .

apn:Shopping a owl:Class ;
    rdfs:label "Shopping" ;
    rdfs:subClassOf apn:ApplicationType .

apn:Social a owl:Class ;
    rdfs:label "Social" ;
    skos:definition "Notifications that encourage the subscriber to engage with social tools e.g. share, like, comment, reply."@en ;
    rdfs:subClassOf apn:ApplicationType,
        apn:CallToAction .

apn:Sports a owl:Class ;
    rdfs:label "Sports" ;
    rdfs:subClassOf apn:ApplicationType .

apn:Strategy a owl:Class ;
    rdfs:label "Strategy" ;
    rdfs:subClassOf apn:ApplicationType .

apn:TravelAndLocal a owl:Class ;
    rdfs:label "Travel And Local" ;
    rdfs:subClassOf apn:ApplicationType .

apn:Indefinitely a owl:Class ;
    rdfs:label "Indefinitely into the future" ;
    skos:definition "The notification is likely to remain relevant indefinitely into the future. It could relevant for months, years or an indefinite amount of time! Only select this category if the notification is not applicable to any of the other categories."@en ;
    rdfs:subClassOf apn:Urgency .

apn:UntilActionTaken a owl:Class ;
    rdfs:label "Until action taken" ;
    skos:definition "The notification is likely only relevant until some action has occurred which makes it no longer relevant or redundant (e.g. a notification asking the user to sign-in is only relevant until the user has signed in. Similarly, a notification which asks the user to claim their reward is only relevant until they have claimed their reward)."@en ;
    rdfs:subClassOf apn:Urgency .

apn:VideoPlayersAndEditors a owl:Class ;
    rdfs:label "Video Players And Editors" ;
    rdfs:subClassOf apn:ApplicationType .

apn:Watch a owl:Class ;
    rdfs:label "Watch" ;
    skos:definition "Notifications that encourage the user to watch some content on the application."@en ;
    rdfs:subClassOf apn:CallToAction .

apn:WatchApps a owl:Class ;
    rdfs:label "Watch Apps" ;
    rdfs:subClassOf apn:ApplicationType .

apn:WatchFaces a owl:Class ;
    rdfs:label "Watch Faces" ;
    rdfs:subClassOf apn:ApplicationType .

apn:Weather a owl:Class ;
    rdfs:label "Weather" ;
    rdfs:subClassOf apn:ApplicationType .

apn:Word a owl:Class ;
    rdfs:label "Word" ;
    rdfs:subClassOf apn:ApplicationType .

apn:accountCreated a owl:DatatypeProperty ;
    rdfs:label "account created" ;
    skos:definition "User created an account to use the application."@en ;
    rdfs:domain apn:Application ;
    rdfs:range xsd:boolean .

apn:appName a owl:DatatypeProperty ;
    rdfs:label "app name" ;
    skos:definition "The name of the application"@en ;
    rdfs:domain apn:Application ;
    rdfs:range xsd:string .

apn:canBeUsedToInfer a owl:ObjectProperty ;
    rdfs:label "can be used to infer" ;
    skos:definition "Indicates the type of personal data that can be inferred from the notification."@en ;
    rdfs:domain apn:PushNotification ;
    rdfs:range apn:Personalisation .

apn:hasAppType a owl:ObjectProperty ;
    rdfs:label "has app type" ;
    skos:definition "Indicates the application type"@en ;
    rdfs:domain apn:Application ;
    rdfs:range apn:ApplicationType .

apn:hasCTA a owl:ObjectProperty ;
    rdfs:label "has call-to-action" ;
    skos:definition "Indicates the call to action of the notification"@en ;
    rdfs:domain apn:PushNotification ;
    rdfs:range apn:CallToAction .

apn:hasCampaignType a owl:ObjectProperty ;
    rdfs:label "has campaign type" ;
    skos:definition "Indicates the campaign type of the notification"@en ;
    rdfs:domain apn:PushNotification ;
    rdfs:range apn:CampaignType .

apn:hasTargetAudience a owl:ObjectProperty ;
    rdfs:label "has target audience" ;
    skos:definition "Indicates the target audience of the notification"@en ;
    rdfs:domain apn:PushNotification ;
    rdfs:range apn:TargetAudience .

apn:inAppPurchases a owl:DatatypeProperty ;
    rdfs:label "in app purchases" ;
    skos:definition "Indicates if the application includes paid features/services"@en ;
    rdfs:domain apn:Application ;
    rdfs:range xsd:boolean .

apn:installDate a owl:DatatypeProperty ;
    rdfs:label "install date" ;
    skos:definition "Indicates the date and time when the application was installed"@en ;
    rdfs:domain apn:Application ;
    rdfs:range xsd:dateTime .

apn:isTimeSensitive a owl:DatatypeProperty ;
    rdfs:label "is time sensitive" ;
    skos:definition "Indicates weather the notification is urgent, i.e. time-sensitive, or not."@en ;
    rdfs:domain apn:PushNotification ;
    rdfs:range xsd:boolean .

apn:notificationID a owl:DatatypeProperty ;
    rdfs:label "notification ID" ;
    skos:definition "Unique identifier of the notification"@en ;
    rdfs:domain apn:PushNotification ;
    rdfs:range xsd:integer .

apn:notificationText a owl:DatatypeProperty ;
    rdfs:label "notification text" ;
    skos:definition "Text content of the notification, including emojis"@en ;
    rdfs:domain apn:PushNotification ;
    rdfs:range xsd:string .

apn:numberOfDownloads a owl:DatatypeProperty ;
    rdfs:label "number of downloads" ;
    skos:definition "Indicates the number of times that the application was downloaded"@en ;
    rdfs:domain apn:Application ;
    rdfs:range xsd:integer .

apn:numberOfReviews a owl:DatatypeProperty ;
    rdfs:label "number of reviews" ;
    skos:definition "Indicates the number of reviews that the application has on the app store"@en ;
    rdfs:domain apn:Application ;
    rdfs:range xsd:integer .

apn:pushedBy a owl:ObjectProperty ;
    rdfs:label "pushed by" ;
    skos:definition "Indicates the app that pushed the notification"@en ;
    rdfs:domain apn:PushNotification ;
    rdfs:range apn:Application .

apn:pushedOn a owl:DatatypeProperty ;
    rdfs:label "pushed on" ;
    skos:definition "Date and time when the notification is pushed by the application"@en ;
    rdfs:domain apn:PushNotification ;
    rdfs:range xsd:dateTime .

apn:remainsRelevant a owl:ObjectProperty ;
    rdfs:label "remains relevant" ;
    skos:definition "Indicates the urgency of the notification - the period of time when the notification remains relevant for the user"@en ;
    rdfs:domain apn:PushNotification ;
    rdfs:range apn:Urgency .

apn:requiresAccount a owl:DatatypeProperty ;
    rdfs:label "requires account" ;
    skos:definition "Indicates if the application requires the creation of an account to use"@en ;
    rdfs:domain apn:Application ;
    rdfs:range xsd:boolean .

apn:sizeInMB a owl:DatatypeProperty ;
    rdfs:label "size in MB" ;
    skos:definition "Indicates the size of the application in megabytes"@en ;
    rdfs:domain apn:Application ;
    rdfs:range xsd:float .

apn:stars a owl:DatatypeProperty ;
    rdfs:label "stars" ;
    skos:definition "Indicates the mean number of stars given by the users to the application"@en ;
    rdfs:domain apn:Application ;
    rdfs:range xsd:float .

apn:Application a owl:Class ;
    rdfs:label "Application" ;
    skos:definition "Computer program or software application designed to run on a mobile device such as a phone, tablet, or watch. Mobile applications often stand in contrast to desktop applications which are designed to run on desktop computers, and web applications which run in mobile web browsers rather than directly on the mobile device."@en .

apn:Geographic a owl:Class ;
    rdfs:label "Geographic" ;
    skos:definition "Targeting users based on their geographic whereabouts."@en ;
    rdfs:subClassOf apn:TargetAudience .

apn:CT_Promotional a owl:Class ;
    rdfs:label "Campaign Type: Promotional" ;
    skos:definition "A campaign based on promotional offers for the users."@en ;
    rdfs:subClassOf apn:CampaignType .

apn:Psychographic a owl:Class ;
    rdfs:label "Psychographic" ;
    skos:definition "Targeting users based on their interests, personal motivations or lifestyle."@en ;
    rdfs:subClassOf apn:TargetAudience .

apn:Demographic a owl:Class ;
    rdfs:label "Demographic" ;
    skos:definition "Targeting users based on quantifiable characteristics such as family status or job experience. "@en ;
    rdfs:subClassOf apn:TargetAudience .

apn:Behavior a owl:Class ;
    rdfs:label "Behavior" ;
    skos:definition "Targeting users based on their behavior, purchase intent and interaction with certain online services or products."@en ;
    rdfs:subClassOf apn:TargetAudience .

apn:TargetAudience a owl:Class ;
    rdfs:label "Target Audience" ;
    skos:definition "Indicates the audience being targeted by the notification, based on their behavior or other demographic, geographic or psychographic characteristics."@en .

apn:PushNotification a owl:Class ;
    skos:definition "Push notifications are pop-up messages, sent by mobile or browser applications, that appear on the users’ devices. Subscribers can be anywhere and still receive these messages as long as they’re online or have their browsers running on their devices."@en ;
    rdfs:label "Push Notification" .

apn:Urgency a owl:Class ;
    rdfs:label "Urgency" ;
    skos:definition "The urgency of the notification - if it contains information that is only relevant for a certain period of time and becomes redundant if that period of time passes (for example, a notification about Friday night is irrelevant if delivered on Saturday morning)."@en .

apn:CampaignType a owl:Class ;
    rdfs:label "Campaign Type" ;
    skos:definition "Indicates the campaign type of the notification, based on the marketing strategy followed by a company to keeps its brand's visibility, i.e., to mantain and increase the number of notification subscribers."@en .

apn:CallToAction a owl:Class ;
    rdfs:label "Call To Action" ;
    skos:definition "The call-to-action of the notification - for example, 'Anne sent you a message on App X' is encouraging the user to interact with the app to communicate with other people."@en .

apn:Personalisation a owl:Class ;
    rdfs:label "Personalisation" ;
    skos:definition "Indicates personal information that can be derived or inferred from the notification."@en .

apn:ApplicationType a owl:Class ;
    rdfs:label "Application Type" ;
    skos:definition ""@en .

